added detProds

Taskin/Binarize.thy
@@ -1,5 +1,5 @@
 theory Binarize
-imports "../CFG"
+imports "../CFG" detProds
 begin
 
 (* FFPI *)
@@ -33,8 +33,6 @@ proof -
   from this[of "m x"] show ?thesis using assms[of "(f ^^ m x) x"] by auto
 qed
 
-(* definition of binarize *)
-
 fun binarize1 :: "('n :: infinite, 't) prods \<Rightarrow> ('n, 't) prods \<Rightarrow> ('n, 't) prods" where
   "binarize1 ps' [] = []"
 | "binarize1 ps' ((A, []) # ps) = (A, []) # binarize1 ps' ps"
@@ -51,8 +49,6 @@ fun count :: "('n::infinite, 't) prods \<Rightarrow> nat" where
 
 definition binarize :: "('n::infinite, 't) prods \<Rightarrow> ('n, 't) prods" where
   "binarize ps = (binarize' ^^ (count ps)) ps"
-
-(* fixed point iteration*)
 
 lemma count_dec1:
   assumes "binarize1 ps' ps \<noteq> ps" 
@@ -92,8 +88,6 @@ proof -
   then show ?thesis using funpow_fix by metis
 qed
 
-(* proof for binary productions only *)
-
 lemma binarize_binary1: 
   assumes "ps = binarize1 ps' ps"
   shows "(A,w) \<in> set(binarize1 ps' ps) \<Longrightarrow> length w \<le> 2"
@@ -129,295 +123,6 @@ lemma binarize_binary':
 lemma length_binarize: "(A,w) \<in> set(binarize ps) \<Longrightarrow> length w \<le> 2"
   unfolding binarize_def using binarize_ffpi binarize_binary' by metis
 
-(* definitions for inlining *)
-
-fun substW :: "'a list \<Rightarrow> 'a \<Rightarrow> 'a list \<Rightarrow> 'a list" where
-  "substW [] _ _ = []"
-| "substW (x#xs) y ys = (if x = y then ys @ substW xs y ys else x # substW xs y ys)"
-
-(* facts about substW *)
-(* may be unnecesarry *)
-
-lemma substW_split: "substW (xs @ xs') y ys = substW xs y ys @ substW xs' y ys"
-  by (induction xs) auto
-
-lemma substW_skip: "y \<notin> set xs \<Longrightarrow> substW xs y ys = xs"
-  by (induction xs) auto
-
-lemma substW_len: "length (substW xs y [y']) = length xs"
-  by (induction xs) auto
-
-lemma substW_rev: "y' \<notin> set xs \<Longrightarrow> substW (substW xs y [y']) y' [y] = xs"
-  by (induction xs) auto
-
-(* refine *)
-lemma substW_der:
-  "(B,v) \<in> set ps \<Longrightarrow> (set ps) \<turnstile> u \<Rightarrow>* substW u (Nt B) v"
-proof (induction u)
-  case Nil
-  then show ?case by simp
-next
-  case (Cons a u)
-  then show ?case
-    by (metis (no_types, lifting) derivel_Nt_Cons derivel_imp_derive derives_Cons rtranclp.rtrancl_into_rtrancl substW.simps(2))
-qed
-
-(* inlining *)
-definition substP :: "('n::infinite, 't) prods \<Rightarrow>  ('n, 't) sym \<Rightarrow>  ('n, 't) syms \<Rightarrow> ('n, 't) prods" where
-  "substP ps s u = map (\<lambda>(A,v). (A, substW v s u)) ps"
-
-(* domain *)
-fun dom :: "('n::infinite, 't) prods \<Rightarrow> 'n list" where
-  "dom [] = []"
-| "dom ((A,u) # ps) = A # dom ps"
-
-(* symbols *)
-fun syms :: "('n::infinite, 't) prods \<Rightarrow> ('n,'t) syms" where
-  "syms [] = []"
-| "syms ((A,v)#ps) = Nt A # v @ syms ps"
-
-lemma syms_inv:
-  "s \<in> set (syms ps) \<longleftrightarrow> (\<exists>A u. (A,u) \<in> set ps \<and> (s = Nt A \<or> s \<in> set u))"
-proof
-  assume "s \<in> set (syms ps)"
-  then show "\<exists>A u. (A, u) \<in> set ps \<and> (s = Nt A \<or> s \<in> set u)"
-  proof (induction ps)
-    case Nil
-    then show ?case by simp
-  next
-    case (Cons a ps)
-    let ?A = "fst a" let ?u = "snd a"
-    have A_u_set: "(?A, ?u) \<in> set (a # ps)" by simp
-    then show ?case proof (cases "s \<in> set (syms ps)")
-      case True
-      then show ?thesis using Cons.IH by auto
-    next
-      case False
-      with Cons.prems have "s \<in> set (Nt ?A # ?u)" 
-        by (metis (no_types, opaque_lifting) Un_iff append_eq_Cons_conv set_append split_pairs syms.simps(2))
-      then have "(s = Nt ?A \<or> s \<in> set ?u)" by auto
-      with A_u_set show ?thesis by blast
-    qed
-  qed
-next
-  assume asm: "\<exists>A u. (A, u) \<in> set ps \<and> (s = Nt A \<or> s \<in> set u)"
-  then show "s \<in> set (syms ps)"
-  proof (induction ps)
-    case Nil
-    then show ?case by simp
-  next
-    case (Cons a ps)
-    with asm obtain A u where A_u_def: "(A, u) \<in> set (a # ps) \<and> (s = Nt A \<or> s \<in> set u)" by blast
-    then show ?case proof (cases "(A, u) \<in> set ps")
-      case True
-      with Cons.IH A_u_def show ?thesis
-        by (metis (mono_tags, lifting) Un_iff list.discI list.sel(3) list.set_intros(2) set_append syms.elims)
-    next
-      case False
-      with A_u_def have "(A,u) = a" by simp
-      then show ?thesis
-        using A_u_def by force
-    qed
-  qed
-qed
-
-lemma syms_subset: 
-  "set ps \<subseteq> set ps' \<Longrightarrow> s \<in> set (syms ps) \<Longrightarrow> s \<in> set (syms ps')"
-  by (induction ps) (auto simp add: syms_inv)
-
-(* facts about substP*)
-(* may be unnecesarry *)
-
-lemma substP_split: "substP (ps @ ps') s u = substP ps s u @ substP ps' s u"
-  by (simp add: substP_def)
-
-lemma substP_skip1: "s \<notin> set v \<Longrightarrow> substP ((A,v) # ps) s u = (A,v) # substP ps s u"
-  by (auto simp add: substW_skip substP_def)
-
-lemma substP_skip2: "s \<notin> set (syms ps) \<Longrightarrow> substP ps s u = ps"
-  by (induction ps) (auto simp add: substP_def substW_skip)
-
-lemma substP_rev: "Nt B \<notin> set (syms ps) \<Longrightarrow> substP (substP ps s [Nt B]) (Nt B) [s] = ps"
-proof (induction ps)
-  case Nil
-  then show ?case
-    by (simp add: substP_def)
-next
-  case (Cons a ps)
-  let ?A = "fst a" let ?u = "snd a"
-  have "substP (substP (a # ps) s [Nt B]) (Nt B) [s] = substP (map (\<lambda>(A,v). (A, substW v s [Nt B])) (a#ps)) (Nt B) [s]"
-    by (simp add: substP_def)
-  also have "... = substP ((?A, substW ?u s [Nt B]) # map (\<lambda>(A,v). (A, substW v s [Nt B])) ps) (Nt B) [s]"
-    by (simp add: case_prod_unfold)
-  also have "... = map ((\<lambda>(A,v). (A, substW v (Nt B) [s]))) ((?A, substW ?u s [Nt B]) # map (\<lambda>(A,v). (A, substW v s [Nt B])) ps)"
-    by (simp add: substP_def)
-  also have "... = (?A, substW (substW ?u s [Nt B]) (Nt B) [s]) # substP (substP ps s [Nt B]) (Nt B) [s]"
-    by (simp add: substP_def)
-  also from Cons have "... = (?A, substW (substW ?u s [Nt B]) (Nt B) [s]) # ps"
-    using syms_subset set_subset_Cons by metis
-  also from Cons.prems have "... = (?A, ?u) # ps"
-    using substW_rev syms_inv by (metis list.set_intros(1) prod.collapse)
-  also have "... = a # ps" by simp
-  finally show ?case by simp
-qed
-
-lemma substP_dom:
-"dom ps = dom (substP ps s u)"
-  by (induction ps) (auto simp add: substP_def)
-
-(* inlining proofs *)
-
-lemma if_set_map:
-  "x' \<in> set (map f l) \<Longrightarrow> (\<exists>x. x \<in> set l \<and> f x = x')"
-  by auto
-
-lemma substP_der:
-  "(A,u) \<in> set (substP ps (Nt B) v) \<Longrightarrow> set ((B,v) # ps) \<turnstile> [Nt A] \<Rightarrow>* u"
-proof -
-  assume "(A,u) \<in> set (substP ps (Nt B) v)"
-  then have "\<exists>u'. (A,u') \<in> set ps \<and> u = substW u' (Nt B) v" 
-    using if_set_map by (smt (verit, del_insts) Pair_inject case_prod_conv old.prod.exhaust substP_def)
-  then obtain u' where u'_def: "(A,u') \<in> set ps \<and> u = substW u' (Nt B) v" by blast
-  then have path1: "set ((B,v) # ps) \<turnstile> [Nt A] \<Rightarrow>* u'"
-    by (simp add: derive_singleton r_into_rtranclp)
-  have "set ((B,v) # ps) \<turnstile> u' \<Rightarrow>* substW u' (Nt B) v"
-    using substW_der by (metis list.set_intros(1))
-  with u'_def have path2: "set ((B,v) # ps) \<turnstile> u' \<Rightarrow>* u" by simp
-  from path1 path2 show ?thesis by simp
-qed
-
-(* refine *)
-lemma if_part:
-  "set (substP ps (Nt B) v) \<turnstile> [Nt A] \<Rightarrow>* u \<Longrightarrow> set ((B,v) # ps) \<turnstile> [Nt A] \<Rightarrow>* u"
-proof (induction rule: rtranclp.induct)
-  case (rtrancl_refl a)
-  then show ?case by simp
-next
-  case (rtrancl_into_rtrancl a b c)
-  then show ?case 
-    using substP_der by (smt (verit, best) derive.simps derives_append derives_prepend rtranclp_trans)
-qed
-
-lemma dom_set: 
-  "B \<notin> set (dom ps) \<Longrightarrow> (B,v) \<notin> set ps"
-by (induction ps) auto
-
-(* refine and rename *)
-lemma subst_P_W: 
-  assumes prem: "set ((B,v)#ps) \<turnstile> nta \<Rightarrow>* u"
-      and NTA_def: "nta = [Nt A]"
-      and A_B_noteq: "A \<noteq> B"
-      and B_notin_dom: "B \<notin> set (dom ps)"
-      and B_notin_v: "Nt B \<notin> set v"
-    shows "set (substP ps (Nt B) v) \<turnstile> nta \<Rightarrow>* substW u (Nt B) v"
-using assms proof (induction rule: rtranclp.induct)
-  case (rtrancl_refl a)
-  then show ?case by simp
-next
-  case (rtrancl_into_rtrancl a b c)
-  then obtain s B' v' w where b_c_def: "b = s @ [Nt B'] @ w \<and> c = s @ v' @ w \<and> (B',v') \<in> set ((B, v) # ps)" 
-    by (meson derive.simps)
-  then show ?case
-  proof (cases "B = B'")
-    case True
-    then have "v = v'" 
-      using B_notin_dom b_c_def dom_set by auto
-    then have "substW b (Nt B) v = substW c (Nt B) v" 
-      using b_c_def B_notin_v True by (simp add: substW_skip substW_split)
-    then show ?thesis
-      using A_B_noteq B_notin_dom B_notin_v rtrancl_into_rtrancl.IH rtrancl_into_rtrancl.prems(1) by argo
-  next
-    case False
-    then have "(B',v') \<in> set ps"
-      using b_c_def by auto
-    then have "(B', substW v' (Nt B) v) \<in> set (substP ps (Nt B) v)"
-      by (metis (no_types, lifting) list.set_map pair_imageI substP_def)
-    with rtrancl_into_rtrancl show ?thesis  
-      by (smt (verit, ccfv_threshold) False b_c_def derive.simps rtranclp.simps substW.simps(1) substW.simps(2) substW_split sym.inject(1))
-  qed
-qed
-
-(* rename *)
-lemma only_if_part: 
-  assumes "set ((B,v)#ps) \<turnstile> [Nt A] \<Rightarrow>* u"
-      and A_B_noteq: "A \<noteq> B"
-      and B_notin_dom: "B \<notin> set (dom ps)"
-      and B_notin_v: "Nt B \<notin> set v"
-      and B_notin_u: "Nt B \<notin> set u"
-    shows "set (substP ps (Nt B) v) \<turnstile> [Nt A] \<Rightarrow>* u"
-  by (metis assms substW_skip subst_P_W)
-
-lemma substP_lang: 
-  assumes "B \<notin> set (dom ps)" and
-          "Nt B \<notin> set v" and
-          "Nt B \<notin> set u" and
-          "A \<noteq> B"
-        shows "set (substP ps (Nt B) v) \<turnstile> [Nt A] \<Rightarrow>* u \<longleftrightarrow> set ((B,v) # ps) \<turnstile> [Nt A] \<Rightarrow>* u"
-  using assms if_part only_if_part by blast
-
-(* Helper lemmas for binarization proofs *)
-
-(* rename *)
-lemma fresh_dom: "B \<notin> nts (set ps) \<Longrightarrow> B \<notin> set (dom ps)"
-  by (induction ps) (auto simp add: nts_def)
-
-(* rename *)
-lemma nt11: "B \<notin> nt u \<Longrightarrow> Nt B \<notin> set u"
-  by (induction u rule: nt.induct) auto
-
-lemma nt12: "Nt B \<notin> set u \<Longrightarrow> B \<notin> nt u"
-  by (induction u rule: nt.induct) auto
-
-(* refine and rename *)
-lemma fresh_sym: "B \<notin> nts (set ps) \<Longrightarrow> (A,u) \<in> set ps \<Longrightarrow> Nt B \<notin> set u"
-  apply (induction ps) 
-   apply simp
-  using nt11 nts_def by fastforce
-
-(* refine and rename *)
-lemma fresh_syms: "B \<notin> nts (set ps) \<Longrightarrow> Nt B \<notin> set (syms ps)"
-  apply (induction ps)
-   apply simp
-  by (metis dom_set fresh_dom fresh_sym sym.inject(1) syms_inv)
-
-(* rename *)
-lemma syms_not_eq: "Nt B \<notin> set (syms ps) \<Longrightarrow> (A,u) \<in> set ps \<Longrightarrow> A \<noteq> B"
-  by (induction ps) auto
-
-(* rename *)
-lemma syms_not_set: "Nt B \<notin> set (syms ps) \<Longrightarrow> (A,u) \<in> set ps \<Longrightarrow> Nt B \<notin> set u"
-  by (induction ps) auto
-
-(* rename *)
-lemma fresh_sym_dom: "Nt B \<notin> set (syms ps) \<Longrightarrow> N \<in> set (dom ps) \<Longrightarrow> N \<noteq> B"
-  by (induction ps) auto
-
-(* rename *)
-lemma syms_dom: "Nt B \<notin> set (syms ps) \<Longrightarrow> B \<notin> set (dom ps)"
-  by (induction ps) auto
-
-(* rename and refine *)
-lemma syms_dom2: "Nt B \<notin> set (syms ps) \<Longrightarrow> set ps' = set ps \<Longrightarrow> B \<notin> set (dom ps')"
-  apply (induction ps) 
-   apply auto
-  by (metis insertE prod.sel(1) prod.sel(2) sym.inject(1) syms_dom syms_inv)
-
-(* rename *)
-lemma dom_eq: "set (dom ((A,u) # ps)) = set (dom ((A,s) # ps))"
-  by auto
-
-(* rename and refine *)
-lemma syms_dom3: "Nt B \<notin> set (syms ps) \<Longrightarrow> set ps' \<subseteq> set ps \<Longrightarrow> Nt B \<notin> set (syms ps')"
-  apply (induction ps')
-   apply auto
-  using syms_not_eq apply blast
-  by (meson syms_not_set)
-
-(* rename *)
-lemma helpppp:"a \<notin> set (syms ps) \<Longrightarrow> (A,u) \<in> set ps \<Longrightarrow> a \<notin> set u"
-  by (induction ps) auto
-
-(* refine *)
 lemma binarize1_cases:
   "binarize1 ps' ps = ps \<or> (\<exists>A ps'' B u s. set ps = {(A, s#u)} \<union> set ps'' \<and> set (binarize1 ps' ps) = {(A,[s,Nt B]),(B,u)} \<union> set ps'' \<and> Nt B \<notin> set (syms ps'))"
 proof (induction ps' ps rule: binarize1.induct)
@@ -468,13 +173,10 @@ next
   qed
 next
   case (5 ps' C s0 v vb vc ps)
-  then show ?case 
-    by (metis Un_insert_left binarize1.simps(5) fresh fresh_syms list.simps(15) sup_bot_left)
+  then show ?case
+    apply simp by (metis fresh fresh_syms list.simps(15))
 qed
 
-(* Binarization proofs for preserving language *)
-
-(* refine *)
 lemma binarize_der1:
   assumes "N \<in> set (dom ps)"
   shows "set ps \<turnstile> [Nt N] \<Rightarrow>* map Tm x \<longleftrightarrow> set (binarize1 ps ps) \<turnstile> [Nt N] \<Rightarrow>* map Tm x"
@@ -485,24 +187,24 @@ next
   case False
   then obtain A ps'' B u s where defs: "set ps = {(A, s # u)} \<union> set ps'' \<and> set (binarize1 ps ps) = {(A, [s, Nt B]), (B, u)} \<union> set ps'' \<and> Nt B \<notin> set (syms ps)"
     by (meson binarize1_cases)
-  from defs have a_notb: "A \<noteq> B" using syms_not_eq by fast
+  from defs have a_not_b: "A \<noteq> B" using syms_not_eq by fast
+  from defs assms have a1: "N \<noteq> B" using syms_dom_not_eq by auto
+  from defs have a2: "Nt B \<notin> set (map Tm x)" by auto
   from defs have a3: "Nt B \<notin> set u" using syms_not_set by fastforce
-  from defs have notB: "Nt B \<notin> set (syms ps'')" using syms_dom3 by auto
+  from defs have "set ps = set ((A, s # u) # ps'')" by simp
+  with defs a_not_b have a4: "B \<notin> set (dom ((A, [s, Nt B]) # ps''))" using syms_dom2 dom_eq by metis
+  from defs have notB: "Nt B \<notin> set (syms ps'')" using syms_subset2 by auto
   then have 1: "set ps = set (substP ((A, [s, Nt B]) # ps'') (Nt B) u)" proof -
     from defs have "set ps = {(A, s # u)} \<union> set ps''" by simp
     also have "... = set ((A, s#u) # ps'')" by simp
     also have "... = set ([(A, s#u)] @ ps'')" by simp
-    also from defs have "... = set ([(A,substW [s, Nt B] (Nt B) u)] @ ps'')" using helpppp by fastforce
+    also from defs have "... = set ([(A,substW [s, Nt B] (Nt B) u)] @ ps'')" using syms_set by fastforce
     also have "... = set ((substP [(A, [s, Nt B])] (Nt B) u) @ ps'')" by (simp add: substP_def)
     also have "... = set ((substP [(A, [s, Nt B])] (Nt B) u) @ substP ps'' (Nt B) u)" using notB by (simp add: substP_skip2)
     also have "... = set (substP ((A, [s, Nt B]) # ps'') (Nt B) u)" by (simp add: substP_def)
     finally show ?thesis by simp
-    qed
+  qed
   from defs have 2: "set (binarize1 ps ps) = set ((A, [s, Nt B]) # (B, u) # ps'')" by auto
-  from defs assms have a1: "N \<noteq> B" using fresh_sym_dom by auto
-  from defs have a2: "Nt B \<notin> set (map Tm x)" by auto
-  from defs have "set ps = set ((A, s # u) # ps'')" by simp
-  with defs a_notb have a4: "B \<notin> set (dom ((A, [s, Nt B]) # ps''))" using syms_dom2 dom_eq by metis
   with 1 2 a1 a2 a3 a4 show ?thesis using substP_lang
     by (smt (verit) insert_commute list.simps(15))
 qed
@@ -512,7 +214,6 @@ lemma binarize_der':
   shows "set ps \<turnstile> [Nt N] \<Rightarrow>* map Tm x \<longleftrightarrow> set (binarize' ps) \<turnstile> [Nt N] \<Rightarrow>* map Tm x"
   unfolding binarize'_def by (simp add: assms binarize_der1)
 
-(* refine *)
 lemma dom_binarize1:
   "set (dom ps) \<subseteq> set (dom (binarize1 ps' ps))"
 proof (induction ps' ps rule: binarize1.induct)
@@ -530,7 +231,7 @@ next
 next
   case (5 ps' A s0 v vb vc ps)
   then show ?case
-    by (metis (mono_tags, opaque_lifting) binarize1.simps(5) dom.simps(2) list.set_intros(1) set_ConsD set_subset_Cons subset_code(1))
+    apply simp by (metis dom.simps(2) list.set_intros(1) list.set_intros(2) subsetI)
 qed
 
 lemma dom_binarize':
@@ -540,8 +241,8 @@ lemma dom_binarize':
 lemma dom_binarize'':
   "set (dom ps) \<subseteq> set (dom ((binarize'^^n) ps))"
   apply (induction n)
-  apply auto
-  using dom_binarize' by blast
+   apply simp
+  using dom_binarize' by auto
 
 lemma binarize_der'': 
   assumes "A \<in> set (dom ps)"
@@ -572,7 +273,6 @@ lemma lang_binarize':
 
 (* Extending assumption from domain to arbitrary non-terminal *)
 
-(* refine *)
 lemma dom_der:
   assumes "N \<notin> set (dom ps)"
   shows "\<nexists>x. set ps \<turnstile> [Nt N] \<Rightarrow>* map Tm x"
@@ -595,7 +295,6 @@ lemma dom_lang:
   shows "lang ps N = {}"
   using dom_der Lang_def assms by fastforce
 
-(* refine *)
 lemma binarize_syms1:
   assumes  "Nt N \<in> set (syms ps)"
     shows  "Nt N \<in> set (syms (binarize1 ps' ps))"
@@ -614,25 +313,9 @@ next
 next
   case (5 ps' A s0 v vb vc ps)
   then show ?case
-    by (metis (no_types, lifting) Un_iff binarize1.simps(5) list.set_intros(1) set_ConsD set_append set_subset_Cons syms.simps(2) syms_not_set syms_subset)
+    apply simp by (metis (no_types, opaque_lifting) list.set_intros(1) list.set_intros(2) syms_inv)
 qed
 
-lemma nts_to_syms: "N \<in> nts (set ps) \<Longrightarrow> Nt N \<in> set (syms ps)"
-  apply (induction ps)
-   apply (auto simp add: nts_def split: prod.splits)
-  apply (meson nt12)
-  done
-
-lemma syms_to_nts: "Nt N \<in> set (syms ps) \<Longrightarrow> N \<in> nts (set ps)"
-  apply (induction ps)
-   apply (auto simp add: nts_def split: prod.splits)
-  apply (meson nt11)
-  done
-
-lemma nts_syms_equI: "N \<in> nts (set ps) \<longleftrightarrow> Nt N \<in> set (syms ps)"
-  using nts_to_syms syms_to_nts by blast
-
-(* refine *)
 lemma binarize_dom1:
   assumes "N \<notin> set (dom ps)"
       and "N \<in> nts (set ps')"
@@ -652,7 +335,7 @@ next
 next
   case (5 ps' A s0 v vb vc ps)
   then show ?case
-    by (metis binarize1.simps(5) dom.simps(2) fresh insert_iff list.simps(15))
+    apply simp by (metis dom.simps(2) fresh set_ConsD)
 qed
 
 lemma binarize_syms_dom1:
@@ -679,7 +362,6 @@ lemma binarize_syms_dom:
     shows "N \<notin> set (dom (binarize ps)) \<and> N \<in> nts (set (binarize ps))"
   unfolding binarize_def using assms binarize_syms_dom'' by blast
 
-(* Final proof *)
 lemma lang_binarize: 
   assumes "N \<in> nts (set ps)"
   shows "lang ps N = lang (binarize ps) N"
