Taskin/detProds.thy
@@ -1,0 +1,297 @@
+theory detProds
+imports "../CFG"
+begin
+
+(* maybe set? *)
+(* CFG? *)
+(* domain *)
+fun dom :: "('n::infinite, 't) prods \<Rightarrow> 'n list" where
+  "dom [] = []"
+| "dom ((A,u) # ps) = A # dom ps"
+
+(* maybe set? *)
+(* CFG? *)
+(* symbols *)
+fun syms :: "('n::infinite, 't) prods \<Rightarrow> ('n,'t) syms" where
+  "syms [] = []"
+| "syms ((A,v)#ps) = Nt A # v @ syms ps"
+
+(* CFG? *)
+lemma dom_eq: "set (dom ((A,u) # ps)) = set (dom ((A,s) # ps))"
+  by auto
+
+(* CFG? *)
+lemma dom_set: 
+  "B \<notin> set (dom ps) \<Longrightarrow> (B,v) \<notin> set ps"
+  by (induction ps) auto
+
+(* CFG? *)
+lemma fresh_dom: "B \<notin> nts (set ps) \<Longrightarrow> B \<notin> set (dom ps)"
+  by (induction ps) (auto simp add: nts_def)
+
+(* CFG? *)
+lemma nt_set1: "B \<notin> nt u \<Longrightarrow> Nt B \<notin> set u"
+  by (induction u rule: nt.induct) auto
+
+(* CFG? *)
+lemma nt_set2: "Nt B \<notin> set u \<Longrightarrow> B \<notin> nt u"
+  by (induction u rule: nt.induct) auto
+
+(* CFG? *)
+lemma nts_to_syms: "N \<in> nts (set ps) \<Longrightarrow> Nt N \<in> set (syms ps)"
+  apply (induction ps)
+   apply (auto simp add: nts_def split: prod.splits)
+  apply (meson nt_set2)
+  done
+
+(* CFG? *)
+lemma syms_to_nts: "Nt N \<in> set (syms ps) \<Longrightarrow> N \<in> nts (set ps)"
+  apply (induction ps)
+   apply (auto simp add: nts_def split: prod.splits)
+  apply (meson nt_set1)
+  done
+
+(* CFG? *)
+lemma nts_syms_equI: "N \<in> nts (set ps) \<longleftrightarrow> Nt N \<in> set (syms ps)"
+  using nts_to_syms syms_to_nts by blast
+
+(* CFG? *)
+lemma fresh_set: "B \<notin> nts (set ps) \<Longrightarrow> (A,u) \<in> set ps \<Longrightarrow> Nt B \<notin> set u"
+  by (induction ps) (auto simp add: nt_set1 nts_def)
+
+(* CFG? *)
+lemma syms_inv:
+  "s \<in> set (syms ps) \<longleftrightarrow> (\<exists>A u. (A,u) \<in> set ps \<and> (s = Nt A \<or> s \<in> set u))"
+proof
+  assume "s \<in> set (syms ps)"
+  then show "\<exists>A u. (A, u) \<in> set ps \<and> (s = Nt A \<or> s \<in> set u)"
+  proof (induction ps)
+    case Nil
+    then show ?case by simp
+  next
+    case (Cons a ps)
+    let ?A = "fst a" let ?u = "snd a"
+    have A_u_set: "(?A, ?u) \<in> set (a # ps)" by simp
+    then show ?case proof (cases "s \<in> set (syms ps)")
+      case True
+      then show ?thesis using Cons.IH by auto
+    next
+      case False
+      with Cons.prems have "s \<in> set (Nt ?A # ?u)" 
+        by (metis (no_types, opaque_lifting) Un_iff append_eq_Cons_conv set_append split_pairs syms.simps(2))
+      then have "(s = Nt ?A \<or> s \<in> set ?u)" by auto
+      with A_u_set show ?thesis by blast
+    qed
+  qed
+next
+  assume asm: "\<exists>A u. (A, u) \<in> set ps \<and> (s = Nt A \<or> s \<in> set u)"
+  then show "s \<in> set (syms ps)"
+  proof (induction ps)
+    case Nil
+    then show ?case by simp
+  next
+    case (Cons a ps)
+    with asm obtain A u where A_u_def: "(A, u) \<in> set (a # ps) \<and> (s = Nt A \<or> s \<in> set u)" by blast
+    then show ?case proof (cases "(A, u) \<in> set ps")
+      case True
+      with Cons.IH A_u_def show ?thesis
+        by (metis (mono_tags, lifting) Un_iff list.discI list.sel(3) list.set_intros(2) set_append syms.elims)
+    next
+      case False
+      with A_u_def have "(A,u) = a" by simp
+      then show ?thesis
+        using A_u_def by force
+    qed
+  qed
+qed
+
+(* CFG? *)
+lemma syms_subset: 
+  "set ps \<subseteq> set ps' \<Longrightarrow> s \<in> set (syms ps) \<Longrightarrow> s \<in> set (syms ps')"
+  using syms_inv by blast
+
+(* CFG? *)
+lemma syms_not_eq: "Nt B \<notin> set (syms ps) \<Longrightarrow> (A,u) \<in> set ps \<Longrightarrow> A \<noteq> B"
+  using syms_inv by blast
+
+(* CFG? *)
+lemma syms_not_set: "Nt B \<notin> set (syms ps) \<Longrightarrow> (A,u) \<in> set ps \<Longrightarrow> Nt B \<notin> set u"
+  using syms_inv by blast
+
+(* CFG? *)
+lemma syms_dom: "Nt B \<notin> set (syms ps) \<Longrightarrow> B \<notin> set (dom ps)"
+  by (induction ps) auto
+
+(* CFG? *)
+lemma syms_dom2: "Nt B \<notin> set (syms ps) \<Longrightarrow> set ps' = set ps \<Longrightarrow> B \<notin> set (dom ps')"
+  by (induction ps)  (auto simp add: syms_dom syms_inv)
+
+(* CFG? *)
+lemma syms_subset2: "Nt B \<notin> set (syms ps) \<Longrightarrow> set ps' \<subseteq> set ps \<Longrightarrow> Nt B \<notin> set (syms ps')"
+  using syms_subset by blast
+
+(* CFG? *)
+lemma syms_set: "a \<notin> set (syms ps) \<Longrightarrow> (A,u) \<in> set ps \<Longrightarrow> a \<notin> set u"
+  using syms_inv by blast
+
+(* CFG? *)
+lemma fresh_syms: "B \<notin> nts (set ps) \<Longrightarrow> Nt B \<notin> set (syms ps)"
+  using dom_set fresh_dom fresh_set syms_inv by fastforce
+
+(* CFG? *)
+lemma syms_dom_not_eq: "Nt B \<notin> set (syms ps) \<Longrightarrow> N \<in> set (dom ps) \<Longrightarrow> N \<noteq> B"
+  using syms_dom2 by blast
+
+fun substW :: "'a list \<Rightarrow> 'a \<Rightarrow> 'a list \<Rightarrow> 'a list" where
+  "substW [] _ _ = []"
+| "substW (x#xs) y ys = (if x = y then ys @ substW xs y ys else x # substW xs y ys)"
+
+(* lemmas about substW *)
+
+lemma substW_split: "substW (xs @ xs') y ys = substW xs y ys @ substW xs' y ys"
+  by (induction xs) auto
+
+lemma substW_skip: "y \<notin> set xs \<Longrightarrow> substW xs y ys = xs"
+  by (induction xs) auto
+
+lemma substW_len: "length (substW xs y [y']) = length xs"
+  by (induction xs) auto
+
+lemma substW_rev: "y' \<notin> set xs \<Longrightarrow> substW (substW xs y [y']) y' [y] = xs"
+  by (induction xs) auto
+
+lemma substW_der:
+  "(B,v) \<in> set ps \<Longrightarrow> (set ps) \<turnstile> u \<Rightarrow>* substW u (Nt B) v"
+proof (induction u)
+  case Nil
+  then show ?case by simp
+next
+  case (Cons a u)
+  then show ?case
+    by (metis (no_types, lifting) derivel_Nt_Cons derivel_imp_derive derives_Cons rtranclp.rtrancl_into_rtrancl substW.simps(2))
+qed
+
+definition substP :: "('n, 't) prods \<Rightarrow>  ('n, 't) sym \<Rightarrow>  ('n, 't) syms \<Rightarrow> ('n, 't) prods" where
+  "substP ps s u = map (\<lambda>(A,v). (A, substW v s u)) ps"
+
+(* lemmas about substP*)
+
+lemma substP_split: "substP (ps @ ps') s u = substP ps s u @ substP ps' s u"
+  by (simp add: substP_def)
+
+lemma substP_skip1: "s \<notin> set v \<Longrightarrow> substP ((A,v) # ps) s u = (A,v) # substP ps s u"
+  by (auto simp add: substW_skip substP_def)
+
+lemma substP_skip2: "s \<notin> set (syms ps) \<Longrightarrow> substP ps s u = ps"
+  by (induction ps) (auto simp add: substP_def substW_skip)
+
+lemma substP_rev: "Nt B \<notin> set (syms ps) \<Longrightarrow> substP (substP ps s [Nt B]) (Nt B) [s] = ps"
+proof (induction ps)
+  case Nil
+  then show ?case
+    by (simp add: substP_def)
+next
+  case (Cons a ps)
+  let ?A = "fst a" let ?u = "snd a"
+  have "substP (substP (a # ps) s [Nt B]) (Nt B) [s] = substP (map (\<lambda>(A,v). (A, substW v s [Nt B])) (a#ps)) (Nt B) [s]"
+    by (simp add: substP_def)
+  also have "... = substP ((?A, substW ?u s [Nt B]) # map (\<lambda>(A,v). (A, substW v s [Nt B])) ps) (Nt B) [s]"
+    by (simp add: case_prod_unfold)
+  also have "... = map ((\<lambda>(A,v). (A, substW v (Nt B) [s]))) ((?A, substW ?u s [Nt B]) # map (\<lambda>(A,v). (A, substW v s [Nt B])) ps)"
+    by (simp add: substP_def)
+  also have "... = (?A, substW (substW ?u s [Nt B]) (Nt B) [s]) # substP (substP ps s [Nt B]) (Nt B) [s]"
+    by (simp add: substP_def)
+  also from Cons have "... = (?A, substW (substW ?u s [Nt B]) (Nt B) [s]) # ps"
+    using syms_subset set_subset_Cons by metis
+  also from Cons.prems have "... = (?A, ?u) # ps"
+    using substW_rev syms_inv by (metis list.set_intros(1) prod.collapse)
+  also have "... = a # ps" by simp
+  finally show ?case by simp
+qed
+
+lemma substP_dom:
+"dom ps = dom (substP ps s u)"
+  by (induction ps) (auto simp add: substP_def)
+
+lemma if_set_map:
+  "x' \<in> set (map f l) \<Longrightarrow> (\<exists>x. x \<in> set l \<and> f x = x')"
+  by auto
+
+lemma substP_der:
+  "(A,u) \<in> set (substP ps (Nt B) v) \<Longrightarrow> set ((B,v) # ps) \<turnstile> [Nt A] \<Rightarrow>* u"
+proof -
+  assume "(A,u) \<in> set (substP ps (Nt B) v)"
+  then have "\<exists>u'. (A,u') \<in> set ps \<and> u = substW u' (Nt B) v" 
+    using if_set_map by (smt (verit, del_insts) Pair_inject case_prod_conv old.prod.exhaust substP_def)
+  then obtain u' where u'_def: "(A,u') \<in> set ps \<and> u = substW u' (Nt B) v" by blast
+  then have path1: "set ((B,v) # ps) \<turnstile> [Nt A] \<Rightarrow>* u'"
+    by (simp add: derive_singleton r_into_rtranclp)
+  have "set ((B,v) # ps) \<turnstile> u' \<Rightarrow>* substW u' (Nt B) v"
+    using substW_der by (metis list.set_intros(1))
+  with u'_def have path2: "set ((B,v) # ps) \<turnstile> u' \<Rightarrow>* u" by simp
+  from path1 path2 show ?thesis by simp
+qed
+
+lemma if_part:
+  "set (substP ps (Nt B) v) \<turnstile> [Nt A] \<Rightarrow>* u \<Longrightarrow> set ((B,v) # ps) \<turnstile> [Nt A] \<Rightarrow>* u"
+proof (induction rule: rtranclp.induct)
+  case (rtrancl_refl a)
+  then show ?case by simp
+next
+  case (rtrancl_into_rtrancl a b c)
+  then show ?case 
+    using substP_der by (smt (verit, best) derive.simps derives_append derives_prepend rtranclp_trans)
+qed
+
+lemma substPW_der: 
+  assumes prem: "set ((B,v)#ps) \<turnstile> nta \<Rightarrow>* u"
+      and NTA_def: "nta = [Nt A]"
+      and A_B_noteq: "A \<noteq> B"
+      and B_notin_dom: "B \<notin> set (dom ps)"
+      and B_notin_v: "Nt B \<notin> set v"
+    shows "set (substP ps (Nt B) v) \<turnstile> nta \<Rightarrow>* substW u (Nt B) v"
+using assms proof (induction rule: rtranclp.induct)
+  case (rtrancl_refl a)
+  then show ?case by simp
+next
+  case (rtrancl_into_rtrancl a b c)
+  then obtain s B' v' w where b_c_def: "b = s @ [Nt B'] @ w \<and> c = s @ v' @ w \<and> (B',v') \<in> set ((B, v) # ps)" 
+    by (meson derive.simps)
+  then show ?case
+  proof (cases "B = B'")
+    case True
+    then have "v = v'" 
+      using B_notin_dom b_c_def dom_set by auto
+    then have "substW b (Nt B) v = substW c (Nt B) v" 
+      using b_c_def B_notin_v True by (simp add: substW_skip substW_split)
+    then show ?thesis
+      using A_B_noteq B_notin_dom B_notin_v rtrancl_into_rtrancl.IH rtrancl_into_rtrancl.prems(1) by argo
+  next
+    case False
+    then have "(B',v') \<in> set ps"
+      using b_c_def by auto
+    then have "(B', substW v' (Nt B) v) \<in> set (substP ps (Nt B) v)"
+      by (metis (no_types, lifting) list.set_map pair_imageI substP_def)
+    with rtrancl_into_rtrancl show ?thesis 
+      by (smt (verit, ccfv_threshold) False b_c_def derive.simps rtranclp.simps substW.simps(1) substW.simps(2) substW_split sym.inject(1))
+  qed
+qed
+
+lemma only_if_part: 
+  assumes "set ((B,v)#ps) \<turnstile> [Nt A] \<Rightarrow>* u"
+      and A_B_noteq: "A \<noteq> B"
+      and B_notin_dom: "B \<notin> set (dom ps)"
+      and B_notin_v: "Nt B \<notin> set v"
+      and B_notin_u: "Nt B \<notin> set u"
+    shows "set (substP ps (Nt B) v) \<turnstile> [Nt A] \<Rightarrow>* u"
+  by (metis assms substW_skip substPW_der)
+
+lemma substP_lang: 
+  assumes "B \<notin> set (dom ps)" and
+          "Nt B \<notin> set v" and
+          "Nt B \<notin> set u" and
+          "A \<noteq> B"
+        shows "set (substP ps (Nt B) v) \<turnstile> [Nt A] \<Rightarrow>* u \<longleftrightarrow> set ((B,v) # ps) \<turnstile> [Nt A] \<Rightarrow>* u"
+  using assms if_part only_if_part by metis
+
+end
